src/lowparse/LowParse.Low.Combinators.fst
@@ -29,3 +29,130 @@ let validate32_nondep_then
     let h' = HST.get () in
     res
   end else false
+
+inline_for_extraction
+let validate_nochk32_nondep_then
+  (#k1: parser_kind)
+  (#t1: Type0)
+  (#p1: parser k1 t1)
+  (p1' : validator_nochk32 p1)
+  (#k2: parser_kind)
+  (#t2: Type0)
+  (#p2: parser k2 t2)
+  (p2' : validator_nochk32 p2)
+: Tot (validator_nochk32 (nondep_then p1 p2))
+= fun (input: pointer buffer8) (len: pointer U32.t) ->
+  p1' input len;
+  p2' input len
+
+inline_for_extraction
+let validate32_synth
+  (#k: parser_kind)
+  (#t1: Type0)
+  (#t2: Type0)
+  (p1: parser k t1)
+  (f2: t1 -> GTot t2)
+  (p1' : validator32 p1)
+  (u: unit {
+    synth_injective f2
+  })
+: Tot (validator32 (parse_synth p1 f2))
+= fun (input: pointer buffer8) (len: pointer U32.t) ->
+  p1' input len
+
+inline_for_extraction
+let validate_nochk32_synth
+  (#k: parser_kind)
+  (#t1: Type0)
+  (#t2: Type0)
+  (p1: parser k t1)
+  (f2: t1 -> GTot t2)
+  (p1' : validator_nochk32 p1)
+  (u: unit {
+    synth_injective f2
+  })
+: Tot (validator_nochk32 (parse_synth p1 f2))
+= fun (input: pointer buffer8) (len: pointer U32.t) ->
+  p1' input len
+
+inline_for_extraction
+let validate32_total_constant_size
+  (#k: parser_kind)
+  (#t: Type0)
+  (p: parser k t)
+  (sz: U32.t)
+  (u: unit {
+    k.parser_kind_high == Some k.parser_kind_low /\
+    k.parser_kind_low == U32.v sz /\
+    k.parser_kind_metadata.parser_kind_metadata_total = true
+  })
+: Tot (validator32 p)
+= fun (input: pointer buffer8) (len: pointer U32.t) ->
+  let len0 = B.index len 0ul in
+  if U32.lt len0 sz
+  then false
+  else begin
+    advance_slice_ptr input len sz;
+    true
+  end
+
+inline_for_extraction
+let validate_nochk32_constant_size
+  (#k: parser_kind)
+  (#t: Type0)
+  (p: parser k t)
+  (sz: U32.t)
+  (u: unit {
+    k.parser_kind_high == Some k.parser_kind_low /\
+    k.parser_kind_low == U32.v sz
+  })
+: Tot (validator_nochk32 p)
+= fun (input: pointer buffer8) (len: pointer U32.t) ->
+  advance_slice_ptr input len sz
+
+inline_for_extraction
+val validate_nochk_truncate32
+  (#k: parser_kind)
+  (#t: Type0)
+  (p: parser k t)
+  (v: validator_nochk32 p)
+  (input: pointer buffer8)
+  (sz: pointer U32.t)
+: HST.Stack unit
+  (requires (fun h ->
+    is_slice_ptr h input sz /\
+    Some? (parse p (B.as_seq h (B.get h input 0)))
+  ))
+  (ensures (fun h _ h' ->
+    B.modifies_2 input sz h h' /\
+    is_slice_ptr h' input sz /\ (
+    let sq = B.as_seq h (B.get h input 0) in
+    let (Some (res, consumed)) = parse p sq in
+    U32.v (B.get h' sz 0) == consumed /\
+    B.get h' input 0 == B.sub (B.get h input 0) 0ul (U32.uint_to_t consumed) /\ (
+    let sq' = B.as_seq h' (B.get h' input 0) in
+    sq' == Seq.slice sq 0 consumed /\
+    parse p sq' == Some (res, (consumed <: nat))
+  ))))
+
+let validate_nochk_truncate32 #k #t p v input sz =
+  let h = HST.get () in
+  let input0 = B.index input 0ul in
+  let sz0 = B.index sz 0ul in
+  v input sz ;
+  let sz1 = B.index sz 0ul in
+  let len' = U32.sub sz0 sz1 in
+  let input' = B.sub input0 0ul len' in
+  B.upd input 0ul input';
+  B.upd sz 0ul len';
+  let h' = HST.get () in
+  let f () : Lemma (
+    let (Some (res, consumed)) = parse p (B.as_seq h (B.get h input 0)) in
+    let ps' = parse p (B.as_seq h' (B.get h' input 0)) in
+    Some? ps' /\ (
+    let (Some (res', consumed')) = ps' in
+    res == res' /\ (consumed <: nat) == (consumed' <: nat)
+  )) =
+    assert (no_lookahead_weak_on p (B.as_seq h (B.get h input 0)) (B.as_seq h' (B.get h' input 0)))
+  in
+  f ()
